One pen-and-paper exercise left for now

lean/LoVe/LoVe05_FunctionalProgramming_ExerciseSheet.lean
@@ -33,13 +33,26 @@ hypothesis is not strong enough. Start by proving the following generalization
 
 theorem reverseAccu_Eq_reverse_append {α : Type} :
     ∀as xs : List α, reverseAccu as xs = reverse xs ++ as :=
-  sorry
+  by
+    intros as xs
+    revert as
+    induction xs with
+    | nil => simp [reverse, reverseAccu]
+    | cons x xs' ihxs => 
+      simp [reverse, reverseAccu]
+      intros as
+      apply ihxs
+   
 
 /- 1.2. Derive the desired equation. -/
 
 theorem reverseAccu_eq_reverse {α : Type} (xs : List α) :
     reverseAccu [] xs = reverse xs :=
-  sorry
+  calc
+  _ = reverse xs ++ [] := reverseAccu_Eq_reverse_append [] xs
+  _ = reverse xs ++ reverse [] := by simp [reverse]
+  _ = reverse ([] ++ xs) := by simp [reverse]
+  _ = reverse xs := by simp
 
 /- 1.3. Prove the following property.
 
@@ -47,7 +60,9 @@ Hint: A one-line inductionless proof is possible. -/
 
 theorem reverseAccu_reverseAccu {α : Type} (xs : List α) :
     reverseAccu [] (reverseAccu [] xs) = xs :=
-  sorry
+  by
+    rw [reverseAccu_eq_reverse, reverseAccu_eq_reverse, reverse_reverse]
+    
 
 /- 1.4. Prove the following theorem by structural induction, as a "paper"
 proof. This is a good exercise to develop a deeper understanding of how
@@ -90,8 +105,10 @@ def drop {α : Type} : ℕ → List α → List α
 To avoid unpleasant surprises in the proofs, we recommend that you follow the
 same recursion pattern as for `drop` above. -/
 
-def take {α : Type} : ℕ → List α → List α :=
-  sorry
+def take {α : Type} : ℕ → List α → List α
+  | 0,     _      => []
+  | _ + 1, []      => []
+  | m + 1, hd :: xs => hd :: take m xs
 
 #eval take 0 [3, 7, 11]   -- expected: []
 #eval take 1 [3, 7, 11]   -- expected: [3]
@@ -106,12 +123,14 @@ Notice that they are registered as simplification rules thanks to the `@[simp]`
 attribute. -/
 
 @[simp] theorem drop_nil {α : Type} :
-    ∀n : ℕ, drop n ([] : List α) = [] :=
-  sorry
+    ∀n : ℕ, drop n ([] : List α) = [] 
+  | 0 => by simp [drop]
+  | _ + 1 => by simp [drop]
 
 @[simp] theorem take_nil {α : Type} :
-    ∀n : ℕ, take n ([] : List α) = [] :=
-  sorry
+    ∀n : ℕ, take n ([] : List α) = [] 
+  | 0 => by simp [take]
+  | _ + 1 => by simp [take]
 
 /- 2.3. Follow the recursion pattern of `drop` and `take` to prove the
 following theorems. In other words, for each theorem, there should be three
@@ -123,15 +142,32 @@ two arguments to `drop`). For the third case, `← add_assoc` might be useful. -
 theorem drop_drop {α : Type} :
     ∀(m n : ℕ) (xs : List α), drop n (drop m xs) = drop (n + m) xs
   | 0,     n, xs      => by rfl
-  -- supply the two missing cases here
+  | _,     n, []      => by simp
+  | m' + 1,n, x::xs  => 
+    by
+      simp [drop]
+      apply drop_drop
+      
 
 theorem take_take {α : Type} :
-    ∀(m : ℕ) (xs : List α), take m (take m xs) = take m xs :=
-  sorry
+    ∀(m : ℕ) (xs : List α), take m (take m xs) = take m xs
+  | 0,     xs      => by rfl
+  | _,      []      => by simp
+  | m' + 1, x::xs  => 
+    by
+      simp [take]
+      apply take_take 
+
 
 theorem take_drop {α : Type} :
-    ∀(n : ℕ) (xs : List α), take n xs ++ drop n xs = xs :=
-  sorry
+    ∀(n : ℕ) (xs : List α), take n xs ++ drop n xs = xs
+  | 0,     xs      => by rfl
+  | _,      []      => by simp
+  | m' + 1, x::xs  => 
+    by
+      simp [drop, take]
+      apply take_drop 
+      
 
 
 /- ## Question 3: A Type of Terms
@@ -143,6 +179,10 @@ theorem take_drop {α : Type} :
             |  `lam` String Term   -- λ-expression (e.g., `λx. t`)
             |  `app` Term Term     -- application (e.g., `t u`) -/
 
+inductive Term where
+  | var : String → Term
+  | lam : String → Term → Term
+  | app : Term → Term → Term
 -- enter your definition here
 
 /- 3.2 (**optional**). Register a textual representation of the type `Term` as
@@ -150,7 +190,9 @@ an instance of the `Repr` type class. Make sure to supply enough parentheses to
 guarantee that the output is unambiguous. -/
 
 def Term.repr : Term → String
--- enter your answer here
+| var s => s
+| lam s t => "(λ" ++ s ++ ". "    ++ Term.repr t ++ ")"
+| app t u => "(" ++ Term.repr t ++ " " ++ Term.repr u ++ ")"
 
 instance Term.Repr : Repr Term :=
   { reprPrec := fun t prec ↦ Term.repr t }
